Projet_SAV_P5.v
@@ -1,0 +1,469 @@
+Add LoadPath "C:\Users\Hp\Documents\Coq" as CoqDirectory.
+Add LoadPath "/Users/samuel/Documents/Documents-L3/PolyCours/S2/Sem/projet_Semantique" as CoqDirectory.
+Load Projet_SAV_P3.
+
+Definition code_correctness: codeBloc -> stack -> Prop := 
+  fun c e => C[ size e]( tau_code c).
+
+  (*
+Fixpoint stack_correctness (s: stack): Prop :=
+  match s with
+    | empty => True 
+    | element (c_0, e_0) tl => (code_correctness c_0 e_0) /\ stack_correctness e_0 /\ stack_correctness tl
+end.*)
+
+Inductive stack_correctness : stack -> Prop :=
+    | empty_is_correct : stack_correctness empty
+    | top_is_correct : forall c_0 : codeBloc, forall e_0 tl : stack,
+        (code_correctness c_0 e_0) -> (stack_correctness e_0) -> (stack_correctness tl)
+        -> stack_correctness (element (c_0, e_0) tl).
+
+Theorem stack_correctness_is_no_free: forall e: stack,
+    stack_correctness e ->  List.Forall (fun t => C[ 0 ]( t )) (tau_stack e).
+Proof.
+    intro e. intro H. 
+    induction H.
+    simpl.
+    auto.
+    
+    simpl.
+    apply List.Forall_cons.
+    2: trivial.
+
+    unfold code_correctness in H.
+
+    rewrite <- tau_stack_length in H.
+
+    pose u := tau_code c_0; fold u; fold u in H.
+    pose l := tau_stack e_0; fold l; fold l in IHstack_correctness1; fold l in H.
+    apply lemma28.
+    trivial.
+    trivial.
+Qed.
+
+
+Definition state_correctness: krivineState -> Prop := 
+  fun ks => match ks with 
+    | (c, e, s) => code_correctness c e /\ stack_correctness e /\ stack_correctness s
+end.
+
+Lemma option_equality_lemma: forall A : Type, forall (a1 a2: A), Some a1 = Some a2 <-> a1 = a2.
+Proof.
+  move => A a1 a2.
+  split.
+  case.
+  trivial.
+  move => H.
+  rewrite H.
+  trivial.
+Qed.
+
+Lemma tuple_eq_is_eq: forall (A B : Type) (a1 a2 : A) (b1 b2 : B),
+      (a1, b1) = (a2, b2) <-> a1 = a2 /\ b1 = b2.
+Proof.
+  move => A B.
+  split; move => H . split.
+  replace a1 with (fst (a1, b1)); replace a2 with (fst (a2, b2)); trivial.
+  rewrite H.
+  trivial.
+  replace b1 with (snd (a1, b1)); replace b2 with (snd (a2, b2)); trivial.
+  rewrite H; trivial.
+  destruct H.
+  rewrite H. rewrite H0.
+  trivial.
+Qed.
+
+Lemma triple_eq_is_eq: forall (A B C: Type) (a1 a2 : A) (b1 b2 : B) (c1 c2 : C),
+  (a1, b1, c1) = (a2, b2, c2) <-> a1 = a2 /\ b1 = b2 /\ c1 = c2.
+  move => A B C.
+  split.
+  move => H.
+  split.
+  replace a1 with (fst (fst ((a1, b1), c1))); replace a2 with (fst (fst ((a2, b2), c2))); trivial.
+  rewrite H; trivial.
+  split.
+  replace b1 with (snd (fst ((a1, b1), c1))); replace b2 with (snd (fst ((a2, b2), c2))); trivial.
+  rewrite H; trivial.
+  replace c1 with (snd ((a1, b1), c1)); replace c2 with (snd ((a2, b2), c2)); trivial.
+  rewrite H; trivial.
+  move => H. destruct H; destruct H0.
+  rewrite H; rewrite H0; rewrite H1.
+  trivial.
+Qed.
+
+Lemma some_triple_to_eq: forall (A B C: Type) (a1 a2: A) (b1 b2: B) (c1 c2: C),
+  Some (a1, b1, c1) = Some (a2, b2, c2) <-> a1 = a2 /\ b1 = b2 /\ c1 = c2.
+Proof.
+  move => A B C a1 a2 b1 b2 c1 c2.
+  split.
+  move => H.
+  apply triple_eq_is_eq; apply option_equality_lemma; trivial.
+  move => H.
+  apply option_equality_lemma; apply triple_eq_is_eq; trivial.
+Qed.
+
+Lemma correctness_propagation: forall (c1 c2: codeBloc), forall (e1 e2 s1 s2: stack),
+  code_correctness c1 e1 /\ stack_correctness e1 /\ stack_correctness s1 /\ Some (c1, e1, s1) = Some (c2, e2, s2) -> code_correctness c2 e2 /\ stack_correctness e2 /\ stack_correctness s2.
+Proof.
+  move => c1 c2 e1 e2 s1 s2 H.
+  destruct H; destruct H0; destruct H1.
+  suff: c1 = c2 /\ e1 = e2 /\ s1 = s2.
+  move => [E1 [E2 E3]].
+  rewrite <- E1; rewrite <- E2; rewrite <- E3.
+  auto.
+  apply some_triple_to_eq.
+  trivial.
+Qed.
+
+Lemma stack_correctness_propagation: forall c: codeBloc, forall (e s : stack), stack_correctness s /\ stack_correctness e /\ code_correctness c e -> stack_correctness (element (c, e) s).
+Proof.
+  move => c e s H.
+  destruct H; destruct H0.
+  simpl.
+  apply top_is_correct; trivial.
+Qed.
+
+Lemma code_correctness_propagation_access: forall n: nat, forall s: stack, forall p: codeBloc * stack, code_correctness (access (S n)) (element p s) -> code_correctness (access n) s.
+Proof.
+  move => n s p.
+  unfold code_correctness; simpl.
+  unfold hasAllFreeVarUnder; simpl.
+  lia.
+Qed.
+
+Lemma code_correctness_propagation_grab: forall (c c0: codeBloc), forall (e s: stack), code_correctness (grab c) s -> code_correctness c (element (c0, e) s).
+Proof.
+  move => c c0 e s.
+  unfold code_correctness; simpl.
+  move => H.
+  replace (S (size s)) with (size s + 1).
+  apply (lemma4 (tau_code c) (size s)).
+  trivial.
+  lia.
+Qed.
+
+Lemma code_correctness_propagation_push1: forall (c1 c2: codeBloc), forall (e: stack), code_correctness (push c1 c2) e -> code_correctness c1 e.
+Proof.
+  move => c1 c2 e.
+  unfold code_correctness.
+  unfold hasAllFreeVarUnder.
+  simpl.
+  move => [H1 H2].
+  trivial.
+Qed.
+
+Lemma code_correctness_propagation_push2: forall (c1 c2: codeBloc), forall (e: stack), code_correctness (push c1 c2) e -> code_correctness c2 e.
+Proof.
+  move => c1 c2 e.
+  unfold code_correctness.
+  unfold hasAllFreeVarUnder.
+  simpl.
+  move => [H1 H2].
+  trivial.
+Qed.
+
+Lemma correctness_preserved: forall ks: krivineState, forall nks: krivineState, state_correctness ks -> (transitionFunction ks = Some nks) -> state_correctness nks.
+Proof.
+  unfold krivineState.
+  move => ks nks.
+  case ks.
+  move => p_0 s_0.
+  case p_0.
+  move => c_0 e_0.
+  case nks; move => p_1 s_1; case p_1; move => c_1 e_1.
+  case c_0; simpl.
+  case e_0; simpl.
+  move => n _.
+  case n; discriminate.
+  move => p_2 s n.
+  case n; simpl.
+  case p_2.
+  move => c s0 H1 Eq.
+  destruct H1 as [H0 [H1 H2]].
+  inversion H1.
+  apply (correctness_propagation c c_1 s0 e_1 s_0 s_1).
+  auto.
+  
+  case p_2.
+  move => c s0 n0 H Eq.
+  destruct H; destruct H0.
+  apply (correctness_propagation (access n0) c_1 s e_1 s_0 s_1).
+  split.
+  pose H4 := code_correctness_propagation_access n0 s (c, s0) H.
+  trivial.
+  inversion H0.
+  auto.
+
+  case s_0.
+  discriminate.
+
+  move => p s c.
+  case p.
+  move => c0 s0.
+  simpl.
+  move => [H [H0 H1]] Eq.
+  apply (correctness_propagation c c_1 (element (c0, s0) e_0) e_1 s s_1).
+  split.
+
+  apply code_correctness_propagation_grab; trivial.
+  inversion H1.
+  split; auto.
+  apply top_is_correct; trivial.
+
+  move => c c0 [H [H0 H1]] Eq.
+  apply (correctness_propagation c0 c_1 e_0 e_1 (element (c, e_0) s_0) s_1).
+  split.
+  apply (code_correctness_propagation_push2 c c0 e_0); trivial.
+  split; trivial.
+  split; trivial.
+  apply stack_correctness_propagation.
+  pose H2 := code_correctness_propagation_push1 c c0 e_0 H.
+  auto.
+Qed.
+
+(*
+Lemma tau_inner_processing_access_0 : forall c0: codeBloc, forall s s2 s3 : stack,
+  (tau_inner (access 0) (element (c0, s2) s3) s) = tau_inner c0 s2 s.
+*)
+
+Lemma tau_inner_beta_red: forall s : stack, forall u v : lambdaTermeN, beta_sred u v -> beta_sred (tau_inner s u) (tau_inner s v).
+Proof.
+    induction s.
+    simpl.
+    trivial.
+    simpl.
+    case p.
+    intro c; intro s0; intro u; intro v; intro H.
+    apply IHs.
+    apply context_red_l.
+    trivial.
+Qed.
+
+
+(*
+Lemma app_red: forall v u t : lambdaTermeN, (beta_sred (app u v) (app t v)) ->  (beta_sred u t) \/ (beta_sred v v /\ u = t).
+Proof.
+    intro v.
+    induction v; intro u; intro t; intro H.
+Admitted.
+
+
+
+
+Lemma beta_red_tau_inner: forall s : stack, forall u v : lambdaTermeN, beta_sred (tau_inner s u) (tau_inner s v) -> beta_sred u v.
+Proof.
+    intro s.
+    induction s.
+    simpl.
+    trivial.
+
+    simpl.
+    case p; clear p.
+    intro c; intro s0; intro u; intro v.
+    pose t := tau_tuple c s0; fold t; fold t.
+    induction t.
+    intro H.
+    pose H0 := IHs (app u (var n)) (app v (var n)) H.
+    inversion H0.
+    simpl.
+    induction t.
+    simpl in H0.
+    inversion H0.
+    rewrite <- H2 in H0; rewrite <- H2 in H.
+    clear H2; clear u.
+    rewrite <- H3 in *; clear H3; clear s0; clear c.
+    rewrite <- H4 in H0.
+
+    Focus 2.
+    trivial.
+    Focus 2.
+    rewrite <- H3 in *; clear H3; clear c; clear s0.
+    clear H5; clear u0.
+    rewrite <- H4 in *; clear H4; clear v.
+    rewrite <- H1 in *; clear H1; clear u.
+    case H0.
+    
+    pose H5 := evaluation t u0.
+    rewrite H4 in H5.
+    rewrite evaluation in H4.
+    case_eq H0.
+    apply (context_red_l u v (tau_tuple c s0)) in H0.
+    elim H0; trivial.
+    destruct H0.
+    inversion H0.
+    suff: beta_red (app (lambda t) (tau_tuple c s0) ) 
+    trivial.
+Qed.
+*)
+
+Require Import Arith.
+Theorem trans_is_beta_reduce: forall ks1 ks2 : krivineState, transitionFunction ks1 = Some ks2 -> state_correctness ks1 -> beta_sred (tau ks1) (tau ks2) \/ tau ks1 = tau ks2.
+Proof.
+  move => ks1 ks2.
+  case ks1; clear ks1.
+  case ks2; clear ks2.
+  move => p s p0 s0.
+  case p; clear p.
+  case p0; clear p0.
+  move => c s1 c0 s2.
+  case c; clear c.
+  move => n.
+  simpl.
+  case n; clear n.
+  case s1; clear s1.
+  discriminate.
+  move => p1 s3.
+  case p1; clear p1.
+  move => c1 s4.
+
+  move => Correct Eq.
+
+  suff: c1 = c0 /\ s4 = s2 /\ s0 = s.
+  2: apply some_triple_to_eq; trivial.
+
+  move => H.
+  destruct H; destruct H0.
+  rewrite H; rewrite H0; rewrite H1.
+
+
+    induction s.
+    simpl.
+
+
+    case s3.
+    auto.
+    move => p2 s.
+    unfold tau_tuple.
+    simpl.
+    auto.
+    auto.
+
+  move => n0; case s1; clear s1.
+  discriminate.
+  move => p1 s3; case p1; clear p1.
+  move => c1 s4.
+  unfold code_correctness.
+  simpl.
+  unfold hasAllFreeVarUnder.
+  simpl.
+  move => Eq [Correct1 [Correct2 Correct3]].
+  suff: access n0 = c0 /\ s3 = s2 /\ s0 = s.
+  2: apply some_triple_to_eq; trivial.
+  move => H.
+  destruct H; destruct H0.
+  rewrite <- H; rewrite <- H0; rewrite <- H1.
+  induction s0.
+  simpl.
+  unfold tau_tuple.
+  unfold tau_code.
+  rewrite (lemma11 (S n0) 0 (tau_stack (element (c1, s4) s3))).
+  lia.
+  rewrite tau_stack_length.
+  simpl.
+  lia.
+  rewrite (lemma11 (n0) 0 (tau_stack s3)).
+  lia.
+  rewrite tau_stack_length.
+  lia.
+  replace (n0 - 0) with n0; try lia.
+  replace (S n0 - 0) with (S n0); try lia.
+
+  simpl.
+  right.
+  apply List.nth_indep.
+  rewrite tau_stack_length.
+  lia.
+
+  simpl in Correct3.
+  case p in Correct3.
+  inversion Correct3.
+
+  simpl.
+  case p.
+  move => c3 s6.
+
+  unfold tau_tuple.
+  simpl.
+  suff : n0 < length (tau_stack s3).
+  move => Ineg.
+  assert (n0 <? length (tau_stack s3) = true) as Eq2.
+  rewrite (PeanoNat.Nat.ltb_lt); trivial.
+  rewrite Eq2.
+  suff : S n0 < S (length (tau_stack s3)).
+  move => Ineg2.
+  assert (S n0 <? S (length (tau_stack s3)) = true) as Eq3.
+  rewrite (PeanoNat.Nat.ltb_lt); trivial.
+  rewrite Eq3.
+  replace (n0 - 0) with n0.
+  right.
+  pose Eq4 := List.nth_indep (tau_stack s3) (var (S n0)) (var n0).
+  suff : n0 < length (tau_stack s3).
+  move => H9.
+  pose Eq5 := Eq4 n0 H9.
+  rewrite Eq5.
+  trivial.
+  trivial.
+  lia.
+  lia.
+  rewrite tau_stack_length.
+  lia.
+
+  move => c.
+  simpl.
+  case s0; clear s0.
+  discriminate.
+  move => p s0.
+  case p; clear p.
+  move => c1 s3.
+  simpl.
+  move => SomeEq H.
+  destruct H; destruct H0.
+
+  suff : c = c0 /\ element (c1, s3) s1 = s2 /\ s0  = s.
+  2: apply some_triple_to_eq; auto.
+  move => [Eq1 [Eq2 Eq3]].
+  rewrite <- Eq1; rewrite <- Eq2; rewrite <- Eq3.
+  clear SomeEq Eq1 Eq2 Eq3.
+  clear c0; clear s; clear s2.
+
+  unfold code_correctness in H.
+  simpl in H.
+
+  left.
+
+  apply tau_inner_beta_red.
+  apply grab_beta_red.
+
+  apply stack_correctness_is_no_free.
+  trivial.
+
+  move => c c1 Eq.
+  suff : c1 = c0 /\ s1 = s2 /\ element (c, s1) s0 = s.
+  2: apply some_triple_to_eq; auto.
+  move => [Eq1 [Eq2 Eq3]] [H [H0 H1]].
+  rewrite <- Eq1 in *; clear Eq1; clear c0.
+  rewrite <- Eq2 in *; clear Eq2; clear s2.
+  rewrite <- Eq3 in *; clear Eq3; clear s.
+  simpl.
+  right.
+  suff : tau_tuple (push c c1) s1 = app (tau_tuple c1 s1) (tau_tuple c s1).
+  auto.
+  unfold tau_tuple.
+  simpl.
+  trivial.
+Qed.
+
+Lemma lambdaTerme_code_correctness : forall u : lambdaTermeN, isClosed u <-> state_correctness (comp_glob u).
+    split.
+    unfold comp_glob.
+    simpl.
+    unfold code_correctness.
+    simpl.
+    unfold isClosed.
+    rewrite <- comp_is_comp_glob.
+    rewrite comp_and_tau.
+    intro H.
+    split; auto.
+    split; apply empty_is_correct.
+
+    unfold state_correctness.
